generational/spec/GC.Gen.Cheney.fsti
@@ -27,6 +27,7 @@ open GC.Spec.Fields
 open GC.Gen.Base
 open GC.Gen.MinorHeap
 open GC.Gen.Promote
+open GC.Gen.PromoteUpdate
 open GC.Gen.Remembered
 
 module AllocLemmas = GC.Spec.Allocator.Lemmas
