generational/spec/GC.Gen.CheneyCorrectness.fst
@@ -12,6 +12,7 @@ open GC.Spec.Fields
 open GC.Gen.Base
 open GC.Gen.MinorHeap
 open GC.Gen.Promote
+open GC.Gen.PromoteUpdate
 open GC.Gen.Cheney
 
 module AllocLemmas = GC.Spec.Allocator.Lemmas
